Updated the new names

driver/Compiler.v
@@ -51,10 +51,10 @@ Require Stacking.
 Require Mach2Mach2.
 Require Asmgen.
 Require PseudoInstructions.
-Require FlatAsmgen.
-Require MClabelgen.
-Require MCcallgen.
-Require MCdatagen.
+Require SegAsmgen.
+Require TAsmlabelgen.
+Require TAsmcallgen.
+Require TAsmdatagen.
 Require FlatMCgen.
 (** Proofs of semantic preservation. *)
 Require SimplExprproof.
@@ -80,11 +80,11 @@ Require Asmgenproof.
 Require RawAsmproof.
 Require RealAsmproof2.
 Require PseudoInstructionsproof.
-Require FlatAsmgenproof.
-Require FlatAsmGlobenv.
-Require FlatAsmProgram.
-Require FlatAsmgen.
-Require FlatAsmSep.
+Require SegAsmgenproof.
+Require SegAsmGlobenv.
+Require SegAsmProgram.
+Require SegAsmgen.
+Require SegAsmSep.
 (* Require MClabelgenproof. *)
 (* Require MClabelsep. *)
 (** Command-line flags. *)
@@ -191,15 +191,15 @@ Definition transf_c_program_real p : res Asm.program :=
   @@@ PseudoInstructions.check_program
   @@ time "Elimination of pseudo instruction" PseudoInstructions.transf_program.
 
-Definition transf_c_program_flatasm p : res FlatAsm.program :=
+Definition transf_c_program_flatasm p : res SegAsm.program :=
   transf_c_program_real p
-  @@@ time "Generation of FlatAsm" FlatAsmgen.transf_program.
+  @@@ time "Generation of SegAsm" SegAsmgen.transf_program.
 
-Definition transf_c_program_mc p : res MC.program :=
+Definition transf_c_program_mc p : res TransSegAsm.program :=
   transf_c_program_flatasm p
-  @@@ time "Generation of relative jumps in MC" MClabelgen.transf_program
-  @@ time "Generation of short calls in MC" MCcallgen.transf_program
-  @@ time "Generation of data addresses in MC" MCdatagen.transf_program.
+  @@@ time "Generation of relative jumps in SegAsm" TAsmlabelgen.transf_program
+  @@ time "Generation of short calls in SegAsm" TAsmcallgen.transf_program
+  @@ time "Generation of data addresses in SegAsm" TAsmdatagen.transf_program.
 
 Definition transf_c_program_fmc p : res FlatMC.program :=
   transf_c_program_mc p
@@ -320,7 +320,7 @@ Definition match_prog_real :=
 
 Definition flat_asm_passes :=
   passes_app real_asm_passes
-             (mkpass FlatAsmgenproof.match_prog ::: pass_nil _).
+             (mkpass SegAsmgenproof.match_prog ::: pass_nil _).
 
 Definition match_prog_flat := 
   pass_match (compose_passes (passes_app CompCert's_passes flat_asm_passes)).
@@ -517,22 +517,22 @@ Definition fn_stack_requirements (tp: Asm.program) (id: ident) : Z :=
   | None => 0
   end.
 
-Definition flat_fn_stack_requirements (tp: FlatAsm.program) (id: ident) : Z :=
-  match List.find (fun '(id',_,_) => ident_eq id id') (FlatAsmProgram.prog_defs tp) with
+Definition flat_fn_stack_requirements (tp: SegAsm.program) (id: ident) : Z :=
+  match List.find (fun '(id',_,_) => ident_eq id id') (SegAsmProgram.prog_defs tp) with
   | None => 0
   | Some (_, def, _) =>
     match def with
-    | Some (Gfun (Internal f)) => FlatAsmProgram.fn_stacksize f
+    | Some (Gfun (Internal f)) => SegAsmProgram.fn_stacksize f
     | _ => 0
     end
   end.
 
-Definition mc_fn_stack_requirements (tp: MC.program) (id: ident) : Z :=
-  match List.find (fun '(id',_,_) => ident_eq id id') (FlatAsmProgram.prog_defs tp) with
+Definition mc_fn_stack_requirements (tp: TransSegAsm.program) (id: ident) : Z :=
+  match List.find (fun '(id',_,_) => ident_eq id id') (SegAsmProgram.prog_defs tp) with
   | None => 0
   | Some (_, def, _) =>
     match def with
-    | Some (Gfun (Internal f)) => FlatAsmProgram.fn_stacksize f
+    | Some (Gfun (Internal f)) => SegAsmProgram.fn_stacksize f
     | _ => 0
     end
   end.
@@ -588,9 +588,9 @@ Definition mk_init_stk {F V} (p: AST.program F V) : StackADT.stack :=
   (Some (StackADT.make_singleton_frame_adt
            (Globalenvs.Genv.genv_next (Globalenvs.Genv.globalenv p)) 0 0), nil) :: nil .
 
-Definition mk_init_stk_flat {I D} (p: @FlatAsmProgram.program I D) : StackADT.stack :=
+Definition mk_init_stk_flat {I D} (p: @SegAsmProgram.program I D) : StackADT.stack :=
   (Some (StackADT.make_singleton_frame_adt
-           (FlatAsmGlobenv.Genv.genv_next (FlatAsmProgram.globalenv p)) 0 0), nil) :: nil .
+           (SegAsmGlobenv.Genv.genv_next (SegAsmProgram.globalenv p)) 0 0), nil) :: nil .
 
 
 Theorem cstrategy_semantic_preservation:
@@ -834,7 +834,7 @@ Proof.
 Qed.
 
 Lemma flat_fn_stack_requirements_match: forall p tp
-    (FM: FlatAsmgenproof.match_prog p tp),
+    (FM: SegAsmgenproof.match_prog p tp),
     fn_stack_requirements p = flat_fn_stack_requirements tp.
 Proof.
   intros.
@@ -844,26 +844,26 @@ Proof.
   destr.
   - unfold Globalenvs.Genv.find_funct_ptr.
     generalize FM. intros FM'.
-    unfold FlatAsmgenproof.match_prog, FlatAsmgen.transf_program in FM'.
+    unfold SegAsmgenproof.match_prog, SegAsmgen.transf_program in FM'.
     repeat destr_in FM'. destruct w.
     exploit Globalenvs.Genv.find_symbol_def_inversion; eauto. intros IN.
-    exploit FlatAsmgenproof.transl_prog_pres_def; eauto.
+    exploit SegAsmgenproof.transl_prog_pres_def; eauto.
     intros (def' & sb & IN' & TLDEF).
-    exploit FlatAsmgenproof.transl_prog_list_norepet; eauto.
+    exploit SegAsmgenproof.transl_prog_list_norepet; eauto.
     intros NPT.
     erewrite find_unique; eauto.
     destruct (Globalenvs.Genv.find_def (Globalenvs.Genv.globalenv p) b) eqn:FDEF.
     destruct g0. destruct f. 
-    monadInv TLDEF. erewrite FlatAsmgenproof.transl_fun_pres_stacksize; eauto.
+    monadInv TLDEF. erewrite SegAsmgenproof.transl_fun_pres_stacksize; eauto.
     monadInv TLDEF. auto.
-    FlatAsmgenproof.monadInvX TLDEF. auto.
+    SegAsmgenproof.monadInvX TLDEF. auto.
     monadInv TLDEF. auto.
   - assert (~ In i (prog_defs_names p)). 
     eapply Globalenvs.Genv.find_symbol_inversion_none; eauto.
-    unfold FlatAsmgenproof.match_prog, FlatAsmgen.transf_program in FM.
+    unfold SegAsmgenproof.match_prog, SegAsmgen.transf_program in FM.
     repeat destr_in FM. 
-    assert (~ exists def sb, In (i, def, sb) (FlatAsmProgram.prog_defs tp)).
-    eapply FlatAsmgenproof.transl_prog_pres_non_def; eauto.
+    assert (~ exists def sb, In (i, def, sb) (SegAsmProgram.prog_defs tp)).
+    eapply SegAsmgenproof.transl_prog_pres_non_def; eauto.
     destr. apply find_some in Heqo0. destruct p0. destruct p0.
     destruct Heqo0. exfalso. apply H0. destruct ident_eq. 
     subst. do 2 eexists; eauto. inv H3.
@@ -872,7 +872,7 @@ Qed.
 Theorem c_semantic_preservation_flat:
   forall p tp,
     match_prog_flat p tp ->
-    backward_simulation (Csem.semantics (flat_fn_stack_requirements tp) p) (FlatAsm.semantics tp (Asm.Pregmap.init Values.Vundef)).
+    backward_simulation (Csem.semantics (flat_fn_stack_requirements tp) p) (SegAsm.semantics tp (Asm.Pregmap.init Values.Vundef)).
 Proof.
   intros.
   unfold match_prog_flat in H.
@@ -885,14 +885,14 @@ Proof.
   assert (match_prog_real p pi'). red. 
   apply compose_passes_app. eexists; split; eauto.
   eapply compose_backward_simulation.
-  apply FlatAsm.flat_asm_single_events.
+  apply SegAsm.flat_asm_single_events.
   replace (flat_fn_stack_requirements tp) with (fn_stack_requirements pi').
   apply c_semantic_preservation_real; auto.
   apply flat_fn_stack_requirements_match; auto.
   eapply forward_to_backward_simulation.
-  eapply FlatAsmgenproof.transf_program_correct; eauto.
+  eapply SegAsmgenproof.transf_program_correct; eauto.
   eapply RealAsm.real_asm_receptive.
-  eapply FlatAsm.semantics_determinate.
+  eapply SegAsm.semantics_determinate.
 Qed.
 
 (* Lemma mc_fn_stack_requirements_match: forall p tp *)
@@ -904,7 +904,7 @@ Qed.
 (*   apply Axioms.extensionality. intro i. *)
 (*   unfold MClabelgenproof.match_prog, MClabelgen.transf_program in FM. *)
 (*   repeat destr_in FM. monadInv H0. revert EQ. simpl. *)
-(*   generalize (FlatAsmProgram.prog_defs p) x. clear. *)
+(*   generalize (SegAsmProgram.prog_defs p) x. clear. *)
 (*   induction l; simpl; intros; eauto. inv EQ. simpl. auto. *)
 (*   monadInv EQ. specialize (IHl _ EQ). *)
 (*   destruct a. destruct p0. simpl. simpl in EQ0. *)
@@ -918,40 +918,40 @@ Qed.
 
 Lemma flatasmgen_update_maps_lmap_code:
   forall defs g l d c g' l' d' c',
-    FlatAsmgen.update_maps g l d c defs = (g', l', d', c') ->
-    (forall i lb sb o, l i lb = Some (sb, o) -> sb = FlatAsmProgram.code_segid) ->
+    SegAsmgen.update_maps g l d c defs = (g', l', d', c') ->
+    (forall i lb sb o, l i lb = Some (sb, o) -> sb = SegAsmProgram.code_segid) ->
     forall i lb sb o,
-      l' i lb = Some (sb, o) -> sb = FlatAsmProgram.code_segid.
+      l' i lb = Some (sb, o) -> sb = SegAsmProgram.code_segid.
 Proof.
   intros defs g l d c g' l' d' c' H H0.
   change ((fun g l d c =>
            forall (i lb : ident) (sb : Segment.segid_type) (o : Integers.Ptrofs.int),
-  l i lb = Some (sb, o) -> sb = FlatAsmProgram.code_segid
+  l i lb = Some (sb, o) -> sb = SegAsmProgram.code_segid
 ) g' l' d' c').
-  eapply FlatAsmgenproof.umind. eauto. auto.
+  eapply SegAsmgenproof.umind. eauto. auto.
   clear. intros.
-  unfold FlatAsmgen.update_maps_def in H.
+  unfold SegAsmgen.update_maps_def in H.
   repeat destr_in H; eauto.
   clear H1. revert l c i l' z Heqp H0 H2.
   generalize (Asm.fn_code f0). clear.
   induction c; simpl; intros; eauto. inv Heqp. eauto.
-  rewrite FlatAsmgenproof.update_instrs_cons in Heqp. destr_in Heqp.
+  rewrite SegAsmgenproof.update_instrs_cons in Heqp. destr_in Heqp.
   specialize (IHc _ _ _ _ _ Heqp).
   eapply IHc; eauto.
   clear - Heqp0 H0.
-  unfold FlatAsmgen.update_instr in Heqp0. inv Heqp0. intros. destr_in H.
-  unfold FlatAsmgen.update_label_map in H. repeat destr_in H; eauto.
+  unfold SegAsmgen.update_instr in Heqp0. inv Heqp0. intros. destr_in H.
+  unfold SegAsmgen.update_label_map in H. repeat destr_in H; eauto.
   eauto.
 Qed.
 
 Lemma flatasmgen_make_maps_code:
   forall p g l d c,
-    FlatAsmgen.make_maps p = (g, l, d, c) ->
+    SegAsmgen.make_maps p = (g, l, d, c) ->
     forall i lb sb o,
-      l i lb = Some (sb, o) -> sb = FlatAsmProgram.code_segid.
+      l i lb = Some (sb, o) -> sb = SegAsmProgram.code_segid.
 Proof.
-  unfold FlatAsmgen.make_maps.
-  intros. eapply flatasmgen_update_maps_lmap_code; eauto. unfold FlatAsmgen.default_label_map.
+  unfold SegAsmgen.make_maps.
+  intros. eapply flatasmgen_update_maps_lmap_code; eauto. unfold SegAsmgen.default_label_map.
   congruence.
 Qed.
 
@@ -979,10 +979,10 @@ Qed.
 (*   eapply MClabelgenproof.transf_program_correct; eauto. *)
 (*   unfold flat_asm_passes in RP. simpl in RP. *)
 (*   destruct RP as (p2 & PI & p3 & PIP & p4 & FAP & EQ). subst. *)
-(*   unfold FlatAsmgenproof.match_prog, FlatAsmgen.transf_program in FAP. *)
-(*   repeat destr_in FAP. unfold FlatAsmgen.transl_prog_with_map in H1. monadInv H1. simpl. *)
+(*   unfold SegAsmgenproof.match_prog, SegAsmgen.transf_program in FAP. *)
+(*   repeat destr_in FAP. unfold SegAsmgen.transl_prog_with_map in H1. monadInv H1. simpl. *)
 (*   clear - Heqp0. eapply flatasmgen_make_maps_code; eauto. *)
-(*   eapply FlatAsm.flat_asm_receptive. *)
+(*   eapply SegAsm.flat_asm_receptive. *)
 (*   eapply MC.semantics_determinate. *)
 (* Qed. *)
 
@@ -1029,7 +1029,7 @@ Qed.
 Theorem transf_c_program_correct_flat:
   forall p tp,
     transf_c_program_flatasm p = OK tp ->
-    backward_simulation (Csem.semantics (flat_fn_stack_requirements tp) p) (FlatAsm.semantics tp (Asm.Pregmap.init Values.Vundef)).
+    backward_simulation (Csem.semantics (flat_fn_stack_requirements tp) p) (SegAsm.semantics tp (Asm.Pregmap.init Values.Vundef)).
 Proof.
   intros. apply c_semantic_preservation_flat. apply transf_c_program_flat_match; auto.
 Qed.
@@ -1124,7 +1124,7 @@ Theorem separate_transf_c_program_correct_flat:
       link_list asm_units = Some asm_program
       /\
       let init_stk := mk_init_stk_flat asm_program in
-      backward_simulation (Csem.semantics (flat_fn_stack_requirements asm_program) c_program) (FlatAsm.semantics asm_program
+      backward_simulation (Csem.semantics (flat_fn_stack_requirements asm_program) c_program) (SegAsm.semantics asm_program
                                                                                                            (Asm.Pregmap.init Values.Vundef)
                                                                                          ).
 Proof.
