x86/FlatMCgen.v
@@ -1,9 +1,9 @@
 Require Import Coqlib Integers AST Maps.
-Require Import Asm MC Segment.
+Require Import Asm TransSegAsm Segment.
 Require Import Errors.
-Require Import FlatAsmBuiltin.
+Require Import SegAsmBuiltin.
 Require Import Memtype.
-Require Import FlatAsmProgram FlatMCProgram FlatMC.
+Require Import SegAsmProgram FlatMCProgram FlatMC.
 Import ListNotations.
 
 Local Open Scope error_monad_scope.
@@ -43,73 +43,73 @@ Definition transl_addr_mode (m: addrmode') : res addrmode :=
     OK (Addrmode b index disp)
   end.
 
-Definition transl_instr (i: MC.instruction) : res instruction :=
+Definition transl_instr (i: TransSegAsm.instruction) : res instruction :=
   match i with
-  | MCjmp_l ofs => OK (FMCjmp_l ofs)
-  | MCjcc c ofs => OK (FMCjcc c ofs)
-  | MCshortcall ofs sg => OK (FMCshortcall ofs sg)
-  | MCleal ofs a => 
+  | TAjmp_l ofs => OK (FMCjmp_l ofs)
+  | TAjcc c ofs => OK (FMCjcc c ofs)
+  | TAshortcall ofs sg => OK (FMCshortcall ofs sg)
+  | TAleal ofs a => 
     do a' <- transl_addr_mode a;
       OK (FMCleal ofs a')
-  | MCAsminstr (Paddl_ri rd n) =>
+  | TAsminstr (Paddl_ri rd n) =>
     OK (FMCaddl_ri rd n)
-  | MCAsminstr (Psubl_ri rd n) =>
+  | TAsminstr (Psubl_ri rd n) =>
     OK (FMCsubl_ri rd n)
-  | MCAsminstr (Psubl_rr rd r1) =>
+  | TAsminstr (Psubl_rr rd r1) =>
     OK (FMCsubl_rr rd r1)
-  | MCAsminstr (Pmovl_ri rd n) =>
+  | TAsminstr (Pmovl_ri rd n) =>
     OK (FMCmovl_ri rd n)
-  | MCAsminstr (Pmov_rr rd r1) =>
+  | TAsminstr (Pmov_rr rd r1) =>
     OK (FMCmov_rr rd r1)
-  | MCmovl_rm rd a =>
+  | TAmovl_rm rd a =>
     do a' <- transl_addr_mode a;
       OK (FMCmovl_rm rd a')
-  | MCmovl_mr a rs =>
+  | TAmovl_mr a rs =>
     do a' <- transl_addr_mode a;
       OK (FMCmovl_mr a' rs)
-  | MCmov_rs rd (sid,sofs) =>
+  | TAmov_rs rd (sid,sofs) =>
     do ofs <- 
        match smap sid with
        | None => Error (msg "Invalid segment in the argument of MCmov_rs")
        | Some ofs => OK (Ptrofs.add ofs sofs)
        end;
       OK (FMCmovl_rm rd (Addrmode None None ofs))
-  | MCmov_rm_a rd a =>
+  | TAmov_rm_a rd a =>
     do a' <- transl_addr_mode a;
       OK (FMCmov_rm_a rd a')
-  | MCmov_mr_a a rs =>
+  | TAmov_mr_a a rs =>
     do a' <- transl_addr_mode a;
       OK (FMCmov_mr_a a' rs)
-  | MCAsminstr (Ptestl_rr r1 r2) =>
+  | TAsminstr (Ptestl_rr r1 r2) =>
     OK (FMCtestl_rr r1 r2)
-  | MCAsminstr (Pret) =>
+  | TAsminstr (Pret) =>
     OK FMCret 
-  | MCAsminstr (Pimull_rr rd r1) =>
+  | TAsminstr (Pimull_rr rd r1) =>
     OK (FMCimull_rr rd r1)
-  | MCAsminstr (Pimull_ri rd n) =>
+  | TAsminstr (Pimull_ri rd n) =>
     OK (FMCimull_ri rd n)
-  | MCAsminstr (Pcmpl_rr r1 r2) =>
+  | TAsminstr (Pcmpl_rr r1 r2) =>
     OK (FMCcmpl_rr r1 r2)
-  | MCAsminstr (Pcmpl_ri r1 n) =>
+  | TAsminstr (Pcmpl_ri r1 n) =>
     OK (FMCcmpl_ri r1 n)
-  | MCAsminstr (Pcltd) =>
+  | TAsminstr (Pcltd) =>
     OK FMCcltd
-  | MCAsminstr (Pidivl r1) =>
+  | TAsminstr (Pidivl r1) =>
     OK (FMCidivl r1)
-  | MCAsminstr (Psall_ri rd n) =>
+  | TAsminstr (Psall_ri rd n) =>
     OK (FMCsall_ri rd n)
-  | MCAsminstr (Plabel l) =>
+  | TAsminstr (Plabel l) =>
     OK FMCnop
   | _ => Error (msg "Instruction not supported")
   end.
 
-Definition transl_instr' (ii: MC.instr_with_info) : res instr_with_info :=
+Definition transl_instr' (ii: TransSegAsm.instr_with_info) : res instr_with_info :=
   let '(i, sb, fid) := ii in
   do i' <- transl_instr i;
     OK (i', segblock_size sb).
 
 (** Translation of a sequence of instructions in a function *)
-Fixpoint transl_instrs (instrs: list MC.instr_with_info) : res (list instr_with_info) :=
+Fixpoint transl_instrs (instrs: list TransSegAsm.instr_with_info) : res (list instr_with_info) :=
   match instrs with
   | nil => OK nil
   | i::instrs' =>
@@ -119,21 +119,21 @@ Fixpoint transl_instrs (instrs: list MC.instr_with_info) : res (list instr_with_
   end.
 
 (** Tranlsation of a function *)
-Definition transl_fun (f:@FlatAsmProgram.function MC.instruction) : res function :=
-  do code' <- transl_instrs (FlatAsmProgram.fn_code f);
-  let sb := (FlatAsmProgram.fn_range f) in
+Definition transl_fun (f:TransSegAsm.function) : res function :=
+  do code' <- transl_instrs (SegAsmProgram.fn_code f);
+  let sb := (SegAsmProgram.fn_range f) in
   match smap (segblock_id sb) with
   | None =>
     Error (msg "Segment block of a function is unkown")
   | Some ofs => 
-    OK (mkfunction (FlatAsmProgram.fn_sig f) code' 
+    OK (mkfunction (SegAsmProgram.fn_sig f) code' 
                    (Ptrofs.add ofs (segblock_start sb))
                    (segblock_size sb))
   end.
 
 
-Definition transl_globdef (def: (ident * option MC.gdef) * segblock) 
-  : res (ident * option (@FlatMCProgram.gdef FlatMC.instr_with_info)) :=
+Definition transl_globdef (def: (ident * option TransSegAsm.gdef) * segblock) 
+  : res (ident * option FlatMC.gdef) :=
   let '(id,def,sb) := def in
   match def with
   | Some (AST.Gfun (Internal f)) =>
@@ -168,12 +168,12 @@ Definition seg_map : SMAP_TYPE :=
     None.
 
 (** Translation of a program *)
-Definition transf_program (p:MC.program) : res program := 
-  do defs <- transl_globdefs seg_map (FlatAsmProgram.prog_defs p);
+Definition transf_program (p:TransSegAsm.program) : res program := 
+  do defs <- transl_globdefs seg_map (SegAsmProgram.prog_defs p);
   OK (Build_program
         defs
-        (FlatAsmProgram.prog_public p)
-        (FlatAsmProgram.prog_main p)
+        (SegAsmProgram.prog_public p)
+        (SegAsmProgram.prog_main p)
         Ptrofs.zero
         Ptrofs.zero
         (segsize (data_seg p))
