Makefile
@@ -111,7 +111,7 @@ BACKEND=\
   Segment.v \
   SegMemAccessors.v SegAsm.v SegAsmGlobenv.v SegAsmBuiltin.v SegAsmProgram.v \
   SegAsmgen.v SegAsmgenproof.v SegAsmSep.v \
-  MC.v MClabelgen.v MCcallgen.v MCdatagen.v \
+  TransSegAsm.v TAsmlabelgen.v TAsmcallgen.v TAsmdatagen.v \
   FlatMCProgram.v FlatMC.v FlatMCgen.v \
   FlatBinary.v FlatBingen.v \
   ValidLabel.v Hex.v Bits.v
